src/tls/Hashing.fst
@@ -17,17 +17,13 @@ let content #a v =
   match v with Inputs b -> b
 
 val start: a:alg -> Tot (v:accv a {content v == empty_bytes})
-val extend: #a: alg -> v: accv a -> 
-  b: bytes {length (content v) + length b <= maxLength a} -> 
-  v': accv a {content v' == content v @| b}
+val extend: #a:alg -> v:accv a -> b:bytes -> Tot (v':accv a {length (content v) + length b = length (content v') /\  content v' == content v @| b})
 val finalize: #a:alg -> v:accv a -> ST (t:tag a {t == hash a (content v)})
   (requires (fun h0 -> True))
   (ensures (fun h0 t h1 -> modifies Set.empty h0 h1))
 
 let start a = Inputs empty_bytes
-let extend #a (Inputs b0) b1 = 
-  assert(length b0 + length b1 <= pow2 32);
-  Inputs (b0 @| b1)
+let extend #a (Inputs b0) b1 = assume (FStar.UInt.fits (length b0 + length b1) 32); Inputs (b0 @| b1)
 let finalize #a (Inputs b) = Hashing.OpenSSL.compute a b
 
 let compute =  Hashing.OpenSSL.compute 
